fold clean code generation into src/Mail/MailServer.v
generates clean code for [ms_bottom_server]; need to tweak the codegen
ltac to generate code for [ms_bottom] which is the benchmark workload.

src/Mail/MailServer.v
@@ -1,4 +1,6 @@
 Require Import CSPEC.
+Require Import Morphisms.
+Require Import FunctionalExtensionality.
 
 Require Import MailServerAPI.
 
@@ -309,3 +311,183 @@ Definition ms_bottom_server nsmtp npop3 :=
   thread_to_list (c0.compile_ts (mail_server nsmtp npop3)).
 
 Print Assumptions c0.compile_traces_match.
+
+
+(**
+ * Generating optimized code.
+ *)
+
+Global Instance SpawnN_exec_equiv_proper :
+  forall Op State T op_step,
+    Proper (eq ==> (@exec_equiv Op State op_step T) ==> exec_equiv_rx op_step) SpawnN.
+Proof.
+  unfold Proper, respectful; intros; subst.
+  induction y; simpl.
+  - reflexivity.
+  - rewrite H0.
+    setoid_rewrite IHy.
+    reflexivity.
+Qed.
+
+Theorem compile_SpawnN :
+  forall Op1 Op2 (compile_op : forall T, Op1 T -> proc Op2 T) n `(p : proc _ T),
+    Compile.compile compile_op (SpawnN n p) =
+    SpawnN n (Compile.compile compile_op p).
+Proof.
+  induction n; simpl; intros; eauto.
+  f_equal.
+  apply functional_extensionality; eauto.
+Qed.
+
+Definition read_list_compiled {Op} (compile_op : forall T, MailboxOp.Op T -> proc Op T) :=
+  fix read_list_compiled' (l : list (nat*nat)) (r : list ((nat*nat) * string)) {struct l} :=
+    match l with
+    | nil =>
+      Compile.compile compile_op ( _ <- Call MailboxOp.Unlock; Ret r )
+    | fn :: l' =>
+      m <- Compile.compile compile_op ( Call (MailboxOp.Read fn) );
+      match m with
+      | None => read_list_compiled' l' r
+      | Some s => read_list_compiled' l' (r ++ ((fn, s) :: nil))
+      end
+    end.
+
+Theorem compile_read_list1 :
+  forall l r,
+    AtomicReader'.read_list l r =
+    read_list_compiled (fun T op => Call op) l r.
+Proof.
+  induction l; simpl; eauto; intros.
+Qed.
+
+Theorem compile_read_list2 :
+  forall Op1 Op2
+         (compile_op1 : forall T, MailboxOp.Op T -> proc Op1 T)
+         (compile_op2 : forall T, Op1 T -> proc Op2 T) l r,
+    Compile.compile compile_op2 (read_list_compiled compile_op1 l r) =
+    read_list_compiled (fun T op => Compile.compile compile_op2 (compile_op1 _ op)) l r.
+Proof.
+  induction l; simpl; eauto; intros.
+  f_equal.
+  apply functional_extensionality; intros.
+  destruct x; eauto.
+Qed.
+
+Definition ms_bottom_server_opt' a b :
+    {ts : threads_state _ | exec_equiv_ts MailFSMergedAPI.step ts
+                            (c0.compile_ts (mail_server a b))}.
+
+  eexists.
+
+  unfold c0.compile_ts.
+  unfold c10.compile_ts.
+  unfold c9.compile_ts.
+  unfold c8.compile_ts.
+  unfold c7.compile_ts.
+  unfold c6.compile_ts.
+  unfold c5'.compile_ts.
+  unfold c4'.compile_ts.
+  unfold c3.compile_ts.
+  unfold c2.compile_ts.
+  unfold c1.compile_ts.
+
+  unfold MailServerComposedImpl.MailServerComposedImpl.compile_ts.
+  unfold MailServerLockAbsImpl.MailServerLockAbsImplH.compile_ts.
+  unfold MailboxImpl.AtomicReaderH.compile_ts.
+  unfold MailboxTmpAbsImpl.MailboxTmpAbsImplH.compile_ts.
+  unfold DeliverImpl.AtomicDeliverH.compile_ts.
+  unfold LinkRetryImpl.LinkRetryImplH.compile_ts.
+  unfold TryDeliverImpl.TryDeliverImplH.compile_ts.
+  unfold MailFSStringAbsImpl.MailFSStringAbsImplH.compile_ts.
+  unfold MailFSStringImpl.MailFSStringImplH.compile_ts.
+  unfold MailFSPathAbsImpl.MailFSPathAbsImplH.compile_ts.
+  unfold MailFSPathImpl.MailFSPathImplH.compile_ts.
+  unfold MailFSMergedImpl.MailFSMergedImpl.compile_ts.
+  unfold MailFSMergedImpl.MailFSMergedOpImpl.compile_ts.
+  unfold MailFSMergedImpl.MailFSMergedAbsImpl.compile_ts.
+
+  unfold compile_ts.
+  unfold Compile.compile_ts.
+  unfold compile.
+
+  autorewrite with t.
+
+  unfold mail_server.
+  unfold threads_from_proc.
+  rewrite thread_map_thread_from_list.
+  cbn [map].
+
+  eapply exec_equiv_ts_thread_from_list.
+
+  eapply Forall2_cons.
+  {
+    do 3 eexists.
+    split; [ reflexivity | ].
+    split; [ reflexivity | ].
+
+    (* Optimize stuff. *)
+    Ltac reflexivity_maybe_fun :=
+      reflexivity ||
+      ( instantiate (1 := fun _ => _); reflexivity ).
+
+    Ltac step :=
+      match goal with
+      | _ => progress simpl; idtac "simpl"
+      (* Fixpoints where [simpl] is not sufficient. *)
+      | |- context[SpawnN] => rewrite compile_SpawnN; idtac "compile SpawnN"
+      | |- context[MailboxImpl.AtomicReader'.read_list] => rewrite compile_read_list1; idtac "compile read_list"
+      | |- context[read_list_compiled] => rewrite compile_read_list2; idtac "compile read_list_compiled"
+      | |- context[read_list_compiled] => unfold read_list_compiled; idtac "unfold read_list_compiled"
+      (* SliceProc is a wrapper around compilation; unfold it. *)
+      | |- context[SliceProc] => unfold SliceProc; idtac "unfold SliceProc"
+      (* Bubble up common program structures. *)
+      | |- exec_equiv _ _ _ => eapply exec_equiv_rx_to_exec_equiv; idtac "exec_equiv_rx"
+      | |- exec_equiv_rx _ _ (Bind _ _) => eapply Bind_exec_equiv_proper; idtac "Bind"
+      | |- exec_equiv_rx _ _ (SpawnN _ _) => eapply SpawnN_exec_equiv_proper; [ reflexivity | ]; idtac "SpawnN"
+      | |- exec_equiv_rx _ _ (Until _ _ _) => rewrite exec_equiv_until_once; idtac "Until once"
+      | |- exec_equiv_rx _ _ (Until _ _ _) => eapply Until_exec_equiv_proper; [ reflexivity_maybe_fun | | reflexivity ]; idtac "Until"
+      (* No more simplifications for [Call] and [Ret]. *)
+      | |- exec_equiv_rx _ _ (Call _) => reflexivity; idtac "Call"
+      | |- exec_equiv_rx _ _ (Ret _) => reflexivity; idtac "Ret"
+      (* Create variables for continuation arguments, if necessary. *)
+      | |- pointwise_relation _ _ _ _ => eapply pointwise_unused; idtac "Unused arg"
+      | |- pointwise_relation _ _ _ _ => eapply pointwise_used; intros; idtac "Used arg"
+      (* Create a [match ..] for things that depend on an argument. *)
+      | |- exec_equiv_rx _ (_ ?arg) ?rhs =>
+        match rhs with
+        | context[match ?arg with _ => _ end] =>
+          idtac "Match on" arg;
+          (
+            instantiate (1 := fun z => match z with | None => _ | Some a => _ a end) ||
+            instantiate (1 := fun z => match z with | (a, b) => _ a b end) ||
+            instantiate (1 := fun z => match z with | exist _ a _ => _ a end) ||
+            instantiate (1 := fun z => match z with | Missing => _ | Present a => _ a end) ||
+            instantiate (1 := fun z => match z with | true => _ | false => _ end) ||
+            instantiate (1 := fun z => match z with
+              | MailServerAPI.MailServerOp.POP3Stat => _
+              | MailServerAPI.MailServerOp.POP3List => _
+              | MailServerAPI.MailServerOp.POP3Retr n => _ n
+              | MailServerAPI.MailServerOp.POP3Delete n => _ n
+              | MailServerAPI.MailServerOp.POP3Closed => _
+              end) ||
+            ( idtac "Could not match on" arg; fail 1 )
+          );
+          idtac "Succeeded in building match on" arg;
+          destruct arg
+        | _ =>
+          instantiate (1 := fun _ => _);
+          idtac "Passing through argument" arg
+        end
+      end.
+
+    repeat step.
+    reflexivity.
+  }
+
+  eapply Forall2_nil.
+Defined.
+
+Definition ms_bottom_server_opt nsmtp npop3 :=
+  Eval cbn in (proj1_sig (ms_bottom_server_opt' nsmtp npop3)).
+
+Print ms_bottom_server_opt.
