src/Spec/CodeOpt.v
@@ -1,0 +1,93 @@
+(**
+ * This file defines helper theorems and tactics to optimize
+ * the code generated through Cspec, by evaluating the layer
+ * compilations before extraction.
+ *)
+
+Require Import Spec.ConcurProc.
+Require Import Spec.ExecSemantics.
+Require Import Spec.Equiv.
+Require Import Spec.ThreadsState.
+Require Import Helpers.ProofAutomation.
+Require Import Helpers.ListStuff.
+Require Import List.
+Require Import Omega.
+Require Import Morphisms.
+
+
+Theorem exec_equiv_ts_thread_from_list' :
+  forall Op State (step : OpSemantics Op State) tl1 tl2 tlbase,
+    Forall2 (fun ep1 ep2 =>
+      exists T p1 p2,
+        ep1 = existT _ T p1 /\
+        ep2 = existT _ T p2 /\
+        exec_equiv step p1 p2) tl1 tl2 ->
+    exec_equiv_ts step (thread_from_list (tlbase ++ tl1))
+                       (thread_from_list (tlbase ++ tl2)).
+Proof.
+  induction tl1; destruct tl2; intros; inversion H; clear H.
+  - reflexivity.
+  - subst; repeat deex.
+    specialize (IHtl1 tl2 (tlbase ++ (existT _ T p2 :: nil)) H5); clear H5.
+    repeat rewrite <- app_assoc in IHtl1; simpl in *.
+    etransitivity; eauto; clear IHtl1.
+    match goal with
+    | |- exec_equiv_ts _ ?ts _ =>
+      specialize (H1 ts (length tlbase))
+    end.
+    repeat rewrite thread_upd_thread_from_list in H1 by
+      ( rewrite app_length; simpl; omega ).
+    repeat rewrite list_upd_app with (l1 := tlbase) in H1 by omega.
+    replace (length tlbase - length tlbase) with 0 in * by omega.
+    simpl in *.
+    eauto.
+Qed.
+
+Theorem exec_equiv_ts_thread_from_list :
+  forall Op State (step : OpSemantics Op State) tl1 tl2,
+    Forall2 (fun ep1 ep2 =>
+      exists T p1 p2,
+        ep1 = existT _ T p1 /\
+        ep2 = existT _ T p2 /\
+        exec_equiv step p1 p2) tl1 tl2 ->
+    exec_equiv_ts step (thread_from_list tl1) (thread_from_list tl2).
+Proof.
+  intros.
+  apply exec_equiv_ts_thread_from_list' with (tlbase := nil).
+  eauto.
+Qed.
+
+Theorem pointwise_unused :
+  forall `(step : OpSemantics Op State) AT RT lhs rhs,
+    exec_equiv_rx step lhs rhs ->
+    pointwise_relation AT (@exec_equiv_rx _ _ step RT)
+      (fun a => lhs) (fun _ => rhs).
+Proof.
+  unfold pointwise_relation; eauto.
+Qed.
+
+Theorem pointwise_used :
+  forall `(step : OpSemantics Op State) AT RT lhs rhs,
+    (forall a, exec_equiv_rx step (lhs a) (rhs a)) ->
+    pointwise_relation AT (@exec_equiv_rx _ _ step RT) lhs rhs.
+Proof.
+  unfold pointwise_relation; eauto.
+Qed.
+
+Theorem exec_equiv_until_once :
+  forall T Op State (step : OpSemantics Op State) (p : proc Op T),
+    exec_equiv_rx
+      step
+      (Until (fun _ => true) (fun _ => p) None)
+      p.
+Proof.
+  intros.
+  rewrite exec_equiv_until.
+  unfold until1.
+  unfold exec_equiv_rx.
+  intros.
+  rewrite exec_equiv_bind_bind.
+  eapply exec_equiv_bind_a; intros.
+  rewrite exec_equiv_ret_bind.
+  reflexivity.
+Qed.
